We are given a fractional equation in a positive variable \(n\). To solve for \(n\), we first multiply both sides of the equation by the denominator:

\[\frac{n-\frac{4n}{n+5}}{\frac{1}{n+5}+\frac{1}{n-5}}=0\]

\(
  \Rightarrow n-\frac{4n}{n+5} = 0\times(\frac{1}{n+5}+\frac{1}{n-5}) = 0
  \\
  \Rightarrow n-\frac{4n}{n+5} = 0
\)

We used the fact that 0 multiplied by any finite number gives itself. can now add the fractions obtained in the regular way, taking a common denominator and appropriately multiplying the numerators:

\(
n-\frac{4n}{n+5} = \frac{n(n+5)}{n+5} - \frac{4n}{n+5} = \frac{n^2 +5n - 4n}{n+5} = \frac{n^2 - n}{n+5}
\\ 
\Rightarrow n-\frac{4n}{n+5} = \frac{n^2 - n}{n+5} = 0
\)

As \(n+5\) appears in the denominator, we must ensure that it never becomes 0.\\ 
Thus, \(n+5 \neq 0 \Rightarrow n \neq -5\). Having said this, we can now multiply \(n+5\) to both sides of the equation to obtain:

\(n^2 - n = 0 \times (n+5) = 0
\\
\Rightarrow n^2 - n = (n)\times(n-1)=0
\\
\Rightarrow n=0 \text{ OR } n-1 = 0
\\
\Rightarrow n=0 \text{ OR } n=1
\)

Thus, we obtain all possible values of \(n\) as \(n=0\) and \(n=1\).

